meta-theory/pure_eval_lemmasScript.sml
@@ -11,30 +11,6 @@ open pure_expTheory pure_valueTheory pure_evalTheory
 
 val _ = new_theory "pure_eval_lemmas";
 
-(* Premise not necessary, but convenient for drule:ing.
-   TODO: surely this can be derived automatically somehow? *)
-Theorem eval_op_cases:
-  ∀op xs t.
-    eval_op op xs = t ⇒
-    (∃s. op = Cons s) ∨
-    (∃x1 x2 x3. op = If ∧ xs = [x1;x2;x3]) ∨
-    (∃s i x. op = Proj s i ∧ xs = [x]) ∨
-    (∃a. op = AtomOp a) ∨
-    (∃b. op = Lit b ∧ xs = []) ∨
-    (op = If ∧ xs = []) ∨
-    (∃x. op = If ∧ xs = [x]) ∨
-    (∃x1 x2. op = If ∧ xs = [x1;x2]) ∨
-    (∃x1 x2 x3 x4 xs'. op = If ∧ xs = x1::x2::x3::x4::xs') ∨
-    (∃s n. op = IsEq s n ∧ xs = []) ∨
-    (∃s n x. op = IsEq s n ∧ xs = [x]) ∨
-    (∃s n x1 x2 xs'. op = IsEq s n ∧ xs = x1::x2::xs') ∨
-    (∃s i. op = Proj s i ∧ xs = []) ∨
-    (∃s i x1 x2 xs'. op = Proj s i ∧ xs = x1::x2::xs') ∨
-    (∃b x xs'. op = Lit b ∧ xs = x::xs')
-Proof
-  ho_match_mp_tac eval_op_ind >> rw[]
-QED
-
 Theorem eval_eq_Cons_IMP:
   eval x = Constructor s xs ⇒
   ∃ts. eval x = eval (Cons s ts) ∧ MAP eval ts = xs ∧
@@ -98,56 +74,62 @@ Proof
       metis_tac[MEM_EL])
 QED
 
-Theorem eval_to_freevars_SUBSET:
+Theorem eval_wh_to_freevars_SUBSET:
   ∀k e1 v e2 x y.
-    eval_to k e1 = v ∧ y ∈ freevars_v v ⇒
+    eval_wh_to k e1 = v ∧ y ∈ freevars_wh v ⇒
     MEM y (freevars e1)
 Proof
-  ho_match_mp_tac eval_to_ind >> rpt strip_tac
-  >- (rename1 ‘Var’ >> gvs[eval_to_def])
-  >- (rename1 ‘Prim’ >> gs[eval_to_def] >>
-      drule eval_op_cases >> rw[] >>
-      gvs[eval_op_def,AllCaseEqs(),MAP_EQ_CONS,DISJ_IMP_THM,FORALL_AND_THM,
-          MEM_MAP,MEM_FLAT,PULL_EXISTS]
-      >- metis_tac[]
-      >- (rpt(PURE_FULL_CASE_TAC >> gvs[]) >> metis_tac[])
-      >- (gvs[el_def,AllCaseEqs()] >>
-          rpt(PURE_FULL_CASE_TAC >> gvs[]) >>
-          gvs[PULL_EXISTS,MEM_EL] >>
-          metis_tac[])
-      >- (PURE_FULL_CASE_TAC >> gvs[] >>
-          rename1 ‘if XX then _ else _’ >>
-          PURE_FULL_CASE_TAC >> gvs[])
-      >- (gvs[is_eq_def] >>
-          rpt(PURE_FULL_CASE_TAC >> gvs[])))
-  >- (rename1 ‘Lam’ >> gvs[freevars_def,MEM_FILTER,eval_to_def])
+  ho_match_mp_tac eval_wh_to_ind >> rpt strip_tac
+  >- (rename1 ‘Var’ >> gvs[eval_wh_to_def])
+  >- (rename1 ‘Lam’ >> gvs[eval_wh_to_def])
   >- (
-      rename1 ‘App’ >>
-      gvs[freevars_def,MEM_FILTER,eval_to_def] >>
-      rpt(PURE_FULL_CASE_TAC >> gvs[]) >>
-      res_tac >> fs[bind_single_def] >>
-      PURE_FULL_CASE_TAC >> fs[freevars_subst] >>
-      gvs[dest_Closure_def,AllCaseEqs(),MEM_FILTER,PULL_EXISTS]
+      rename1 ‘App’ >> gvs[eval_wh_to_def] >>
+      pop_assum mp_tac >> IF_CASES_TAC >> gvs[] >>
+      rpt (CASE_TAC >> gvs[]) >> rw[] >> res_tac >>
+      Cases_on `eval_wh_to k e1` >> gvs[dest_wh_Closure_def] >>
+      gvs[bind_single_def] >> FULL_CASE_TAC >> gvs[] >>
+      res_tac >> gvs[freevars_subst]
       )
   >- (
-      rename1 ‘Letrec’ >>
-      gvs[freevars_def,MEM_FILTER,MEM_FLAT,MEM_MAP,PULL_EXISTS,eval_to_def] >>
-      PURE_FULL_CASE_TAC >> gvs[] >>
-      first_x_assum drule >> strip_tac >>
-      fs[subst_funs_def,freevars_bind] >>
-      reverse FULL_CASE_TAC >- fs[] >>
-      gvs[MEM_FILTER, FDOM_FUPDATE_LIST, FRANGE_FLOOKUP, PULL_EXISTS] >>
-      gvs[MEM_MAP, FORALL_PROD]
+      rename1 ‘Letrec’ >> gvs[eval_wh_to_def] >>
+      FULL_CASE_TAC >> gvs[] >> res_tac >>
+      gvs[subst_funs_def, freevars_bind] >>
+      last_x_assum drule >> FULL_CASE_TAC >> fs[] >>
+      simp[FDOM_FUPDATE_LIST, MAP_MAP_o, combinTheory.o_DEF, UNCURRY] >>
+      CONV_TAC (DEPTH_CONV ETA_CONV) >> simp[]
+      )
+  >- (
+      rename1 ‘Prim’ >> gs[eval_wh_to_def] >>
+      qpat_x_assum `(if _ then _ else _) = _` mp_tac >>
+      IF_CASES_TAC >> gvs[] >- (rw[] >> gvs[freevars_wh_def]) >>
+      TOP_CASE_TAC >> gvs[] >>
+      gvs[AllCaseEqs(),MAP_EQ_CONS,DISJ_IMP_THM,FORALL_AND_THM] >>
+      rw[] >> gvs[freevars_wh_def, EL_MAP, MEM_MAP, PULL_EXISTS]
+      >- (
+        first_x_assum (qspec_then `EL 1 xs` assume_tac) >> gvs[EL_MEM] >>
+        res_tac >> goal_assum drule >> gvs[EL_MEM]
+        )
+      >- (
+        first_x_assum (qspec_then `EL 2 xs` assume_tac) >> gvs[EL_MEM] >>
+        res_tac >> goal_assum drule >> gvs[EL_MEM]
+        )
+      >- (goal_assum drule >> simp[])
+      >- (
+        Cases_on `xs` >> gvs[PULL_EXISTS] >>
+        first_x_assum irule >> gvs[MEM_MAP, PULL_EXISTS] >>
+        res_tac >>
+        goal_assum (drule_at Any) >> gvs[EL_MEM]
+        )
+      >- (CCONTR_TAC >> gvs[])
       )
 QED
 
-Theorem eval_to_Closure_freevars_SUBSET:
+Theorem eval_wh_to_Closure_freevars_SUBSET:
   ∀k e1 e2 x y.
-    eval_to k e1 = Closure x e2 ∧ MEM y (freevars e2) ⇒
+    eval_wh_to k e1 = wh_Closure x e2 ∧ MEM y (freevars e2) ⇒
     x = y ∨ MEM y (freevars e1)
 Proof
-  rpt strip_tac >> drule eval_to_freevars_SUBSET >>
-  simp[MEM_FILTER] >>
+  rpt strip_tac >> drule eval_wh_to_freevars_SUBSET >> simp[] >>
   metis_tac[]
 QED
 
@@ -155,152 +137,27 @@ Theorem eval_Closure_closed:
   eval e1 = Closure x e2 ∧ closed e1 ⇒
   set(freevars e2) ⊆ {x}
 Proof
-  rw[eval_def,Once gen_v] >>
-  gvs[AllCaseEqs()] >>
-  gvs[v_limit_def,limit_def,AllCaseEqs()] >>
-  gvs[some_def] >>
-  qpat_x_assum ‘_ = _’ mp_tac >>
-  SELECT_ELIM_TAC >>
-  conj_tac >- metis_tac[] >>
-  rw[] >>
-  last_x_assum kall_tac >>
-  first_x_assum(resolve_then (Pos hd) assume_tac LESS_EQ_REFL) >>
-  gvs[v_lookup,AllCaseEqs()] >>
-  drule eval_to_Closure_freevars_SUBSET >>
-  rw[SUBSET_DEF] >>
-  gvs[closed_def]
+  rw[eval_def, v_unfold_def] >>
+  fs[Once gen_v, Once follow_path_def] >>
+  FULL_CASE_TAC >> gvs[eval_wh_def] >>
+  pop_assum mp_tac >> DEEP_INTRO_TAC some_intro >> rw[] >>
+  drule eval_wh_to_freevars_SUBSET >> simp[] >>
+  rw[SUBSET_DEF] >> gvs[closed_def] >>
+  metis_tac[]
 QED
 
 Theorem eval_eq_Diverge:
-  eval x = Diverge ⇔ ∀n. eval_to n x = Diverge
+  eval x = Diverge ⇔ ∀n. eval_wh_to n x = wh_Diverge
 Proof
-  fs [eval_def]
-  \\ once_rewrite_tac [gen_v]
-  \\ fs [AllCaseEqs()]
-  \\ reverse eq_tac \\ rw []
-  THEN1 (qexists_tac ‘0’ \\ fs [v_limit_def,v_lookup])
-  \\ fs [v_limit_def]
-  \\ drule limit_not_default \\ fs []
-  \\ strip_tac \\ pop_assum mp_tac
-  \\ simp [v_lookup,AllCaseEqs()] \\ rw []
-  \\ Cases_on ‘k ≤ n’ \\ res_tac \\ fs []
-  \\ Cases_on ‘eval_to n x = Diverge’ \\ fs []
-  \\ ‘n ≤ k’ by fs []
-  \\ imp_res_tac eval_to_not_diverge_mono
-  \\ metis_tac [LESS_EQ_REFL]
+  fs [eval_def, v_unfold_def]
+  \\ once_rewrite_tac [gen_v, follow_path_def]
+  \\ CASE_TAC \\ CASE_TAC \\ gvs[AllCaseEqs(), follow_path_def, eval_wh_def]
+  \\ pop_assum mp_tac \\ DEEP_INTRO_TAC some_intro \\ rw[]
+  >- (goal_assum drule)
+  >- (goal_assum drule)
+  >- (goal_assum drule)
+  >- (gvs[])
+  >- (goal_assum drule)
 QED
-
-(*
-
-CoInductive Diverges:
-  (∀f x.
-    Diverges (subst_funs f x) ⇒
-    Diverges (Letrec f x))
-  ∧
-  (∀x y.
-    Diverges x ⇒
-    Diverges (App x y))
-  ∧
-  (∀x y s body.
-    eval x = Closure s body ∧
-    Diverges (bind s y body) ⇒
-    Diverges (App x y))
-  ∧
-  (∀s n x.
-    Diverges x ⇒
-    Diverges (IsEq s n x))
-  ∧
-  (∀s i x.
-    Diverges x ⇒
-    Diverges (Proj s i x))
-  ∧
-  (∀s xs y ys x.
-    eval x = eval (Cons s (xs ++ y::ys)) ∧
-    Diverges y ⇒
-    Diverges (Proj s (LENGTH xs) x))
-  ∧
-  (∀x y z.
-    Diverges x ⇒
-    Diverges (If x y z))
-  ∧
-  (∀x y z.
-    Diverges y ∧ eval x = True ⇒
-    Diverges (If x y z))
-  ∧
-  (∀x y z.
-    Diverges z ∧ eval x = False ⇒
-    Diverges (If x y z))
-  ∧
-  (∀a x xs.
-    Diverges x ∧ MEM x xs ⇒
-    Diverges (Prim (AtomOp a) xs))
-End
-
-Triviality LESS_LENGTH_IMP:
-  ∀xs n. n < LENGTH xs ⇒ ∃ys y zs. xs = ys ++ y::zs ∧ LENGTH ys = n
-Proof
-  Induct \\ fs [] \\ Cases_on ‘n’ \\ fs []
-  \\ rw [] \\ res_tac \\ gvs []
-  \\ qexists_tac ‘h::ys’ \\ fs []
-  \\ qexists_tac ‘y’ \\ fs []
-  \\ qexists_tac ‘zs’ \\ fs []
-QED
-
-Theorem Diverges_iff:
-  ∀e. eval e = Diverge ⇔ Diverges e
-Proof
-  rw [] \\ eq_tac
-  THEN1
-   (qid_spec_tac ‘e’
-    \\ ho_match_mp_tac Diverges_coind
-    \\ rw [] \\ reverse (Cases_on ‘e’) \\ fs []
-    \\ TRY (fs [eval_thm] \\ NO_TAC)
-    THEN1
-     (rename [‘eval (App f x)’]
-      \\ gvs [eval_thm,AllCaseEqs()]
-      \\ Cases_on ‘eval f’ \\ fs [dest_Closure_def])
-    \\ rename [‘eval (Prim p xs)’]
-    \\ reverse (Cases_on ‘p’) \\ fs [eval_thm]
-    \\ gvs [eval_Prim,DefnBase.one_line_ify NONE eval_op_def,
-            AllCaseEqs(),MAP_EQ_CONS,is_eq_def,el_def,MEM_MAP]
-    THEN1 (goal_assum (first_assum o mp_then Any mp_tac) \\ fs [])
-    \\ pop_assum (assume_tac o GSYM) \\ fs []
-    \\ drule eval_eq_Cons_IMP
-    \\ fs [eval_thm] \\ rw [] \\ fs []
-    \\ drule LESS_LENGTH_IMP \\ rw [] \\ fs []
-    \\ qexists_tac ‘ys’
-    \\ qexists_tac ‘y’
-    \\ qexists_tac ‘zs’ \\ fs []
-    \\ full_simp_tac std_ss [GSYM APPEND_ASSOC,APPEND]
-    \\ qabbrev_tac ‘qs = MAP eval ys’
-    \\ ‘LENGTH ys = LENGTH qs’ by fs [Abbr‘qs’]
-    \\ fs [EL_LENGTH_APPEND])
-  \\ fs [eval_eq_Diverge,PULL_FORALL]
-  \\ gen_tac \\ qid_spec_tac ‘e’ \\ qid_spec_tac ‘n’
-  \\ ho_match_mp_tac eval_to_ind \\ reverse (rw [])
-  \\ TRY (rename [‘Var’] \\ fs [Once Diverges_cases] \\ NO_TAC)
-  \\ TRY (rename [‘Lam’] \\ fs [Once Diverges_cases] \\ NO_TAC)
-  THEN1
-   (rw [eval_to_def] \\ fs [AND_IMP_INTRO]
-    \\ first_x_assum match_mp_tac
-    \\ last_x_assum mp_tac
-    \\ simp [Once Diverges_cases] \\ fs [])
-  THEN1
-   (rw [eval_to_def] \\ fs [AND_IMP_INTRO]
-    \\ qpat_x_assum ‘Diverges _’ mp_tac
-    \\ simp [Once Diverges_cases] \\ rw []
-    \\ cheat (* true *))
-  \\ qpat_x_assum ‘Diverges _’ mp_tac
-  \\ simp [Once Diverges_cases] \\ rw []
-  THEN1 (fs [eval_to_def,eval_op_def,is_eq_def])
-  THEN1 (fs [eval_to_def,eval_op_def,el_def])
-  THEN1
-   (fs [eval_to_def,eval_op_def,el_def,eval_thm] \\ rw []
-    \\ ‘eval_to n x = Constructor s (MAP eval xs' ++ eval y::MAP eval ys)’ by cheat
-    \\ fs [] \\ cheat (* sigh, not provable, I think *))
-  \\ cheat
-QED
-
-*)
 
 val _ = export_theory();
